Update the architecture and hint interface

books/projects/smtlink/verified/extractor.lisp
@@ -17,6 +17,25 @@
 ;; (defsection SMT-extract
 ;;   :parents (verified)
 
+(define type-decl-p ((term pseudo-termp)
+                     (type-info symbol-symbol-alistp))
+  :returns (ok booleanp)
+  (b* ((term (pseudo-term-fix term))
+       (type-info (symbol-symbol-alist-fix type-info)))
+    (case-match term
+      ((type inner-term) (and (symbolp type)
+                              (symbolp inner-term)
+                              (pseudo-termp inner-term)
+                              (not (null (assoc-equal type type-info)))))
+      (& nil)))
+  ///
+  (more-returns
+   (ok (implies (and ok (pseudo-termp term)
+                     (symbol-symbol-alistp type-info))
+                (and (consp term)
+                     (symbolp (cadr term))))
+       :name implies-of-type-decl-p)))
+
 (define var-equal-p ((term pseudo-termp))
   :returns (ok booleanp)
   (b* ((term (pseudo-term-fix term)))
@@ -35,17 +54,19 @@
 ;;   :true-listp t
 ;;   :pred var-equal-list-p)
 
-(define hypo-p ((term pseudo-termp) (fixinfo smt-fixtype-info-p))
+(define hypo-p ((term pseudo-termp) (type-info symbol-symbol-alistp))
   :returns (ok booleanp)
   (b* ((term (pseudo-term-fix term))
-       (fixinfo (smt-fixtype-info-fix fixinfo)))
-    (or (type-decl-p term fixinfo)
-        (var-equal-p term)))
+       (type-info (symbol-symbol-alist-fix type-info))
+       ((if (type-decl-p term type-info)) t))
+    (var-equal-p term))
   ///
   (more-returns
-   (ok (implies (and ok (pseudo-termp term))
+   (ok (implies (and ok (pseudo-termp term)
+                     (symbol-symbol-alistp type-info))
                 (and (consp term)
                      (symbolp (cadr term))))
+       :hints (("Goal" :in-theory (disable pseudo-termp)))
        :name implies-of-hypo-p)))
 
 (defthm pseudo-term-listp-of-append-of-pseudo-term-listp
@@ -68,30 +89,30 @@
   :hints (("Goal" :in-theory (enable pseudo-term-fix)))
   :flag-local nil
 
-  (define extract-disjunct ((term pseudo-termp) (fixinfo smt-fixtype-info-p))
+  (define extract-disjunct ((term pseudo-termp) (type-info symbol-symbol-alistp))
     :returns (mv (extracted pseudo-term-listp)
                  (new-term pseudo-termp))
     :verify-guards nil
     (b* ((term (pseudo-term-fix term)))
       (cond ((not (consp term)) (mv nil term))
             ((and (equal (car term) 'if) (equal (caddr term) ''t))
-             (b* (((mv decl1 term1) (extract-disjunct (cadr term) fixinfo))
-                  ((mv decl2 term2) (extract-disjunct (cadddr term) fixinfo)))
+             (b* (((mv decl1 term1) (extract-disjunct (cadr term) type-info))
+                  ((mv decl2 term2) (extract-disjunct (cadddr term) type-info)))
                (mv (append decl1 decl2)
                    (cond ((or (equal term1 ''t) (equal term2 ''t)) ''t)
                          ((equal term1 ''nil) term2)
                          ((equal term2 ''nil) term1)
                          (t `(if ,term1 't ,term2))))))
             ((equal (car term) 'not)
-             (b* (((mv decl0 term0) (extract-conjunct (cadr term) fixinfo)))
+             (b* (((mv decl0 term0) (extract-conjunct (cadr term) type-info)))
                (mv decl0
                    (cond ((equal term0 ''nil) ''t)
                          ((equal term0 ''t)   ''nil)
                          (t `(not ,term0))))))
             ((or (equal (car term) 'implies)
                  (and (equal (car term) 'if) (equal (cadddr term) ''t)))
-             (b* (((mv decl1 term1) (extract-conjunct (cadr term) fixinfo))
-                  ((mv decl2 term2) (extract-disjunct (caddr term) fixinfo)))
+             (b* (((mv decl1 term1) (extract-conjunct (cadr term) type-info))
+                  ((mv decl2 term2) (extract-disjunct (caddr term) type-info)))
                (mv (append decl1 decl2)
                    (cond ((or (equal term1 ''nil) (equal term2 ''t)) ''t)
                          ((equal term1 ''t) term2)
@@ -99,36 +120,36 @@
                          (t `(if ,term1 ,term2 't))))))
             (t (mv nil term)))))
 
-  (define extract-conjunct ((term pseudo-termp) (fixinfo smt-fixtype-info-p))
+  (define extract-conjunct ((term pseudo-termp) (type-info symbol-symbol-alistp))
     :returns (mv (extracted pseudo-term-listp)
                  (new-term pseudo-termp))
     :verify-guards nil
     (b* ((term (pseudo-term-fix term)))
       (cond ((not (consp term)) (mv nil term))
             ((and (equal (car term) 'if) (equal (cadddr term) ''nil))
-             (b* (((mv decl1 term1) (extract-conjunct (cadr term) fixinfo))
-                  ((mv decl2 term2) (extract-conjunct (caddr term) fixinfo)))
+             (b* (((mv decl1 term1) (extract-conjunct (cadr term) type-info))
+                  ((mv decl2 term2) (extract-conjunct (caddr term) type-info)))
                (mv (append decl1 decl2)
                    (cond ((or (equal term1 ''nil) (equal term2 ''nil)) ''nil)
                          ((equal term1 ''t) term2)
                          ((equal term2 ''t) term1)
                          (t `(if ,term1 ,term2 'nil))))))
             ((equal (car term) 'not)
-             (b* (((mv decl0 term0) (extract-disjunct (cadr term) fixinfo)))
+             (b* (((mv decl0 term0) (extract-disjunct (cadr term) type-info)))
                (mv decl0
                    (cond ((equal term0 ''nil) ''t)
                          ((equal term0 ''t)   ''nil)
                          (t `(not ,term0))))))
-            ((hypo-p term fixinfo)
+            ((hypo-p term type-info)
              (mv (list term) ''t))
             (t (mv nil term)))))
   )
 
 (verify-guards extract-conjunct)
 
-(define extractor ((term pseudo-termp) (fixinfo smt-fixtype-info-p))
+(define extractor ((term pseudo-termp) (type-info symbol-symbol-alistp))
   :returns (mv (hypo-lst pseudo-term-listp) (theorem pseudo-termp))
-  (extract-disjunct term fixinfo))
+  (extract-disjunct term type-info))
 
 #|
 (extractor '(if (if (equal x2 (binary-+ x0 x1))
@@ -149,32 +170,45 @@
 (defthm-extract-flag
   (defthm correctness-of-extract-disjunct
     (implies (and (pseudo-termp term)
-                  (smt-fixtype-info-p fixinfo)
+                  (symbol-symbol-alistp type-info)
                   (alistp a))
              (b* (((mv hypo-lst new-term)
-                   (extract-disjunct term fixinfo)))
+                   (extract-disjunct term type-info)))
                (iff (ev-smtcp `(if ,(conjoin hypo-lst) ,new-term 't) a)
                     (ev-smtcp term a))))
     :flag extract-disjunct
     :hints ((and stable-under-simplificationp
-                 '(:in-theory (e/d (extract-disjunct extract-conjunct) ())))))
+                 '(:in-theory (e/d (extract-disjunct extract-conjunct)
+                                   (pseudo-term-listp-of-cdr-pseudo-termp
+                                    consp-of-cdr-of-pseudo-lambdap
+                                    default-car default-cdr true-listp
+                                    pseudo-termp pseudo-term-listp))))))
   (defthm correctness-of-extract-conjunct
     (implies (and (pseudo-termp term)
-                  (smt-fixtype-info-p fixinfo)
+                  (symbol-symbol-alistp type-info)
                   (alistp a))
              (b* (((mv hypo-lst new-term)
-                   (extract-conjunct term fixinfo)))
+                   (extract-conjunct term type-info)))
                (iff (ev-smtcp `(if ,(conjoin hypo-lst) ,new-term 'nil) a)
                     (ev-smtcp term a))))
     :flag extract-conjunct
     :hints ((and stable-under-simplificationp
-                 '(:in-theory (e/d (extract-disjunct extract-conjunct) ()))))))
+                 '(:in-theory (e/d (extract-disjunct extract-conjunct)
+                                   (pseudo-term-listp-of-cdr-pseudo-termp
+                                    consp-of-cdr-of-pseudo-lambdap
+                                    default-car default-cdr true-listp
+                                    pseudo-termp pseudo-term-listp))))))
+  :hints (("Goal"
+           :in-theory (disable pseudo-term-listp-of-cdr-pseudo-termp
+                               consp-of-cdr-of-pseudo-lambdap
+                               default-car default-cdr true-listp
+                               pseudo-termp pseudo-term-listp))))
 
 (defthm correctness-of-extractor
   (implies (and (pseudo-termp term)
-                (smt-fixtype-info-p fixinfo)
+                (symbol-symbol-alistp type-info)
                 (alistp a))
-           (b* (((mv hypo-lst new-term) (extractor term fixinfo)))
+           (b* (((mv hypo-lst new-term) (extractor term type-info)))
              (iff (ev-smtcp `(if ,(conjoin hypo-lst) ,new-term 't) a)
                   (ev-smtcp term a))))
   :hints (("Goal"
