books/projects/smtlink/verified/type-options.lisp
@@ -8,136 +8,45 @@
 (in-package "SMT")
 (include-book "xdoc/top" :dir :system)
 (include-book "centaur/fty/top" :dir :system)
+(include-book "clause-processors/term-vars" :dir :system)
 
 (include-book "hint-interface")
 
-(defprod type-tuple
-  ((type symbolp)
-   (neighbour-type symbolp)
-   (formals symbol-listp)
-   (thm symbolp)))
-
-(deflist type-tuple-list
-  :elt-type type-tuple-p
-  :true-listp t)
-
 (defalist type-to-types-alist
   :key-type symbolp
-  :val-type type-tuple-list-p
+  :val-type smt-sub/supertype-list-p
   :true-listp t)
 
 (defthm assoc-equal-of-type-to-types-alist
-  (implies (and (type-to-types-alist-p x)
-                (assoc-equal y x))
-           (and (consp (assoc-equal y x))
-                (type-tuple-list-p (cdr (assoc-equal y x))))))
+  (implies (and (type-to-types-alist-p alst)
+                (assoc-equal x alst))
+           (and (consp (assoc-equal x alst))
+                (smt-sub/supertype-list-p (cdr (assoc-equal x alst))))))
 
 (defprod return-spec
   ((formals symbol-listp)
-   (returns-thm symbolp)
-   (replace-thm symbolp)))
+   (thm symbolp)))
 
 (deflist return-spec-list
   :elt-type return-spec-p
   :true-listp t)
 
-;; (fty::deftypes function-description
-;;   (deftagsum arg-decl
-;;     (:next ((next arg-check-p)))
-;;     (:done ((r return-spec-p))))
-;;   (defalist arg-check
-;;     :key-type symbolp
-;;     :val-type arg-decl-p))
-
-(defalist function-description-alist
+(defalist symbol-return-spec-list-alist
   :key-type symbolp
   :val-type return-spec-list-p
   :true-listp t)
 
-(defthm consp-of-assoc-equal-from-function-description-alist-p
-  (implies (and (function-description-alist-p y)
-                (assoc-equal x y))
-           (and (consp (assoc-equal x y))
-                (return-spec-list-p (cdr (assoc-equal x y))))))
-
-(encapsulate ()
-(local (in-theory (disable (:rewrite default-cdr))))
-
-;; example: alist-term = (integer-integer-alistp x)
-;; fresh-var = y
-;; 1. Generate constraint: y = (alist-to-array-fn x)
-;; 2. Use the theorem to establish (alist-array-equiv x y):
-;; thm: (implies (and (integer-integer-alistp a)
-;;                    (equal b (integer-integer-alist-to-array a)))
-;;               (alist-array-equiv a b))
-(defprod a2a-info
-  ((a2a-fn symbolp) ;; the alist-to-array function
-   (formals symbol-listp)
-   (thm symbolp))) ;; the theorem justifying the equiv relationship
-
-(defoption maybe-a2a-info a2a-info-p)
-
-(defalist alist-info
-  :key-type symbolp ;; the alist type recognizer
-  :val-type a2a-info-p
-  :true-listp t)
-
-(defthm assoc-equal-of-alist-info-p
-  (implies (and (alist-info-p ai)
-                (assoc-equal x ai))
-           (consp (assoc-equal x ai))))
-
-(defthm maybe-of-assoc-equal-of-alist-info-p
-  (implies (alist-info-p ai)
-           (maybe-a2a-info-p (cdr (assoc-equal x ai)))))
-
-(defthm a2a-of-assoc-equal-of-alist-info-p
-  (implies (and (alist-info-p ai)
-                (assoc-equal x ai))
-           (a2a-info-p (cdr (assoc-equal x ai)))))
-
-(defprod equiv
-  ((formal-map symbol-symbol-alistp)
-   (thm symbolp)))
-
-(defthm strip-cars-of-equiv->formal-map
-  (implies (equiv-p x)
-           (symbol-listp (strip-cars (equiv->formal-map x)))))
-
-(defalist alist-array-map
-  :key-type symbolp ;; function name
-  :val-type equiv-p ;; equivalence theorem name
-  :true-listp t)
-
-(defthm assoc-equal-of-alist-array-map-p
-  (implies (and (alist-array-map-p aa)
-                (assoc-equal x aa))
-           (and (consp (assoc-equal x aa))
-                (equiv-p (cdr (assoc-equal x aa))))))
-)
-
-(encapsulate ()
-  (local (in-theory (disable (:rewrite default-cdr)
-                             (:rewrite consp-of-pseudo-lambdap)
-                             (:rewrite
-                              acl2::pseudo-lambdap-of-car-when-pseudo-termp)
-                             (:definition pseudo-termp)
-                             (:rewrite
-                              acl2::true-listp-of-car-when-true-list-listp)
-                             (:definition true-list-listp)
-                             (:rewrite
-                              acl2::true-list-listp-of-cdr-when-true-list-listp)
-                             (:definition true-listp)
-                             (:definition symbol-listp))))
+(defthm assoc-equal-of-symbol-return-spec-list-alist
+  (implies (and (symbol-return-spec-list-alist-p alst)
+                (assoc-equal x alst))
+           (and (consp (assoc-equal x alst))
+                (return-spec-list-p (cdr (assoc-equal x alst))))))
 
 (defprod type-options
   ((supertype type-to-types-alist-p)
    (subtype type-to-types-alist-p)
-   (functions function-description-alist-p)
-   (nil-alst symbol-symbol-alistp)  ;; map from type recognizers to its nil-fn
-   (alist alist-info-p)
-   (aa-map alist-array-map-p)))
-)
+   (functions symbol-return-spec-list-alist-p)
+   (names symbol-listp)))
 
 (define is-type? ((type symbolp)
                   (supertype-alst type-to-types-alist-p))
@@ -146,21 +55,50 @@
        (type (symbol-fix type)))
     (not (null (assoc-equal type supertype-alst)))))
 
-(define is-alist? ((type symbolp)
-                   (options type-options-p))
-  :returns (a2a maybe-a2a-info-p)
-  (b* ((options (type-options-fix options))
-       ((type-options to) options)
-       (yes? (assoc-equal type to.alist)))
-    (cdr yes?)))
+(define construct-sub/supertype-alist ((types smt-type-list-p))
+  :returns (mv (subtype type-to-types-alist-p)
+               (supertype type-to-types-alist-p))
+  :measure (len types)
+  (b* ((types (smt-type-list-fix types))
+       ((unless (consp types)) (mv nil nil))
+       ((cons types-hd types-tl) types)
+       ((smt-type tp) types-hd)
+       ((mv subtype-tl supertype-tl)
+        (construct-sub/supertype-alist types-tl)))
+    (mv (acons tp.recognizer tp.subtypes subtype-tl)
+        (acons tp.recognizer tp.supertypes supertype-tl))))
 
-(define construct-type-options ((smtlink-hint smtlink-hint-p))
+(define construct-return-spec ((formals symbol-listp)
+                               (return-lst symbol-listp))
+  :returns (return-spec-lst return-spec-list-p)
+  :measure (len return-lst)
+  (b* ((formals (symbol-list-fix formals))
+       (return-lst (symbol-list-fix return-lst))
+       ((unless (consp return-lst)) nil)
+       ((cons return-hd return-tl) return-lst))
+    (cons (make-return-spec :formals formals :thm return-hd)
+          (construct-return-spec formals return-tl))))
+
+(define construct-function-alist ((funcs smt-function-list-p))
+  :returns (func-alst symbol-return-spec-list-alist-p)
+  :measure (len funcs)
+  (b* ((funcs (smt-function-list-fix funcs))
+       ((unless (consp funcs)) nil)
+       ((cons f-hd f-tl) funcs)
+       ((smt-function f) f-hd))
+    (acons f.name (construct-return-spec f.formals f.returns)
+           (construct-function-alist f-tl))))
+
+(define construct-type-options ((smtlink-hint smtlink-hint-p)
+                                (term pseudo-termp))
   :returns (type-options type-options-p)
-  :irrelevant-formals-ok t
-  :ignore-ok t
-  (b* ((smtlink-hint (smtlink-hint-fix smtlink-hint)))
-    (make-type-options)))
-
-(defprod type-inference-hints
-  ((type-options type-options-p)
-   (names symbol-listp)))
+  (b* ((smtlink-hint (smtlink-hint-fix smtlink-hint))
+       (term (pseudo-term-fix term))
+       ((smtlink-hint h) smtlink-hint)
+       ((mv subtype supertype) (construct-sub/supertype-alist h.types))
+       (functions (construct-function-alist h.functions))
+       (names (acl2::simple-term-vars term)))
+    (make-type-options :supertype supertype
+                       :subtype subtype
+                       :functions functions
+                       :names names)))
